share/pulse/examples/dice/cbor/COSE.AST.fst
@@ -1,0 +1,26 @@
+module COSE.AST
+open CDDL.Interpreter
+module Spec = COSE.Spec
+
+#push-options "--fuel 0"
+
+[@@  sem_attr]
+let e0 = empty_wf_ast_env
+
+[@@  sem_attr]
+let generic_headers: group NMapGroup =
+  GZeroOrOne (GMapElem () false (TElem (ELiteral (LInt CBOR.Spec.Constants.cbor_major_type_uint64 Spec.h_alg))) tint)
+
+[@@  sem_attr]
+let header_map = TMap generic_headers
+
+let e1 = wf_ast_env_extend_typ
+  e0
+  "header_map"
+  (_ by (solve_by_norm ()))
+  header_map
+  (_ by (solve_mk_wf_typ_fuel_for ()))
+
+irreducible let print (#t: Type) (x: t) : prop = False
+
+// let _ : squash (print (e1.e_wf "header_map"))  = (_ by (solve_by_norm (); FStar.Tactics.fail "abc"))
